{
 "cells": [
  {
   "cell_type": "markdown",
   "metadata": {},
   "source": [
    "## Linear Regression 线性回归模型推导\n"
   ]
  },
  {
   "cell_type": "markdown",
   "metadata": {},
   "source": [
    "#### 最小二乘法推导\n",
    "##### ref: \n",
    "\n",
    "\\begin{align*}\n",
    "L(W) &= \\sum_{i=1}^N \\| W^T x_i - y_i \\|^2 \\\\\n",
    "&= \\sum_{i=1}^N (W^T x_i - y_i)^2 \\\\\n",
    "&= \\left( W^T x_1 - y_1, W^T x_2 - y_2, \\dots, W^T x_N - y_N \\right)( W^T x_1 - y_1, W^T x_2 - y_2, \\dots, W^T x_N - y_N )^T \\\\\n",
    "&= \\left(( W^T x_1, W^T x_2, \\dots, W^T x_N \\right) - \\left( y_1, y_2, \\dots, y_N \\right))( W^T x_1 - y_1, W^T x_2 - y_2, \\dots, W^T x_N - y_N )^T \\\\\n",
    "&= (W^T \\begin{pmatrix} x_1, x_2, \\dots, x_N \\end{pmatrix} - \\begin{pmatrix} y_1, y_2, \\dots, y_N \\end{pmatrix})( W^T x_1 - y_1, W^T x_2 - y_2, \\dots, W^T x_N - y_N )^T \\\\\n",
    "&= (W^T X^T - Y^T)(XW - Y)\\\\\\\\\n",
    "所以 L(w) 通过矩阵求导得出，L(W) &= (W^T X^T - Y^T)(XW - Y) \\\\\n",
    "&= W^T X^T X W - 2 W^T X^T Y + Y^T Y \\\\\n",
    "\\hat{W} &= \\arg \\min L(W) \\\\\n",
    "\\frac{\\partial L(W)}{\\partial W} &= 2 X^T X W - 2 X^T Y = 0\\\\\n",
    "X^TXW &= X^TY\\\\\n",
    "最后得出，W &=(X^TX)^{-1}X^TY\n",
    "\\end{align*}"
   ]
  }
 ],
 "metadata": {
  "language_info": {
   "name": "python"
  }
 },
 "nbformat": 4,
 "nbformat_minor": 2
}
